test/Token.v
@@ -11,3 +11,7 @@ Definition parseToken : parser string :=
 
 Goal parse parseToken "GET / HTTP/1.1" = inr "GET".
 Proof. reflexivity. Qed.
+
+Goal string_of_list_ascii <$>
+     parse (manyN 3 (satisfy isdigit)) "412404 Not Found" = inr "412".
+Proof. reflexivity. Qed.
